theories/Index/Index.v
@@ -9,6 +9,7 @@ Require Import PnV.Math.BooleanAlgebra.
 Require Import PnV.Math.ClassicalDomainTheory.
 Require Import PnV.Math.DomainTheory.
 Require Import PnV.Math.OrderTheory.
+Require Import PnV.Math.ClassicalSetTheory.
 Require Import PnV.Math.SetTheory.
 Require Import PnV.Math.ThN.
 Require Import PnV.Data.Aczel.
